src/ShouldBuild.v
@@ -4,7 +4,7 @@ From Perennial Require Import program_logic.recovery_adequacy.
 From Perennial Require Import program_logic.crash_inv.
 
 From Perennial.go_lang Require Import
-     adequacy total_adequacy lib.spin_lock.
+     adequacy total_adequacy lib.spin_lock encoding.
 (* goose deep output *)
 From Perennial.go_lang.examples Require Import
      goose_unittest append_log wal mailserver simpledb logging2 rfc1813.
