src/go_lang/encoding.v
@@ -1,0 +1,112 @@
+From Perennial.go_lang Require Import lang notation.
+From Perennial.go_lang Require Import struct typing slice.
+
+Section go_lang.
+  Context `{ffi_sem: ext_semantics}.
+  Context {ext_ty:ext_types ext}.
+
+  Set Default Proof Using "ext ext_ty".
+
+  Definition Var' s : @expr ext := Var s.
+  Local Coercion Var' : string >-> expr.
+
+  Definition EncodeUInt32: val :=
+    λ: "n" "p",
+    "p" +ₗ #0 <- to_u8 ("n" ≫ #(U32 $ 0*8));;
+    "p" +ₗ #1 <- to_u8 ("n" ≫ #(U32 $ 1*8));;
+    "p" +ₗ #2 <- to_u8 ("n" ≫ #(U32 $ 2*8));;
+    "p" +ₗ #3 <- to_u8 ("n" ≫ #(U32 $ 3*8)).
+
+  Theorem EncodeUInt32_t : (⊢ EncodeUInt32 : (uint32T -> arrayT byteT -> unitT))%T.
+  Proof.
+    typecheck.
+  Qed.
+
+  Definition DecodeUInt32: val :=
+    λ: "p",
+    to_u32 (!("p" +ₗ #0)) ≪ #(U32 $ 0*8) ∥
+    to_u32 (!("p" +ₗ #1)) ≪ #(U32 $ 1*8) ∥
+    to_u32 (!("p" +ₗ #2)) ≪ #(U32 $ 2*8) ∥
+    to_u32 (!("p" +ₗ #3)) ≪ #(U32 $ 3*8)
+  .
+
+  Theorem DecodeUInt32_t : (⊢ DecodeUInt32 : (arrayT byteT -> uint32T))%T.
+  Proof.
+    typecheck.
+  Qed.
+
+  Definition EncodeUInt64: val :=
+    λ: "n" "p",
+    "p" +ₗ #0 <- to_u8 ("n" ≫ #(0*8));;
+    "p" +ₗ #1 <- to_u8 ("n" ≫ #(1*8));;
+    "p" +ₗ #2 <- to_u8 ("n" ≫ #(2*8));;
+    "p" +ₗ #3 <- to_u8 ("n" ≫ #(3*8));;
+    "p" +ₗ #4 <- to_u8 ("n" ≫ #(4*8));;
+    "p" +ₗ #5 <- to_u8 ("n" ≫ #(5*8));;
+    "p" +ₗ #6 <- to_u8 ("n" ≫ #(6*8));;
+    "p" +ₗ #7 <- to_u8 ("n" ≫ #(7*8))
+  .
+
+  Theorem EncodeUInt64_t : (⊢ EncodeUInt64 : (uint64T -> arrayT byteT -> unitT))%T.
+  Proof.
+    typecheck.
+  Qed.
+
+  Definition DecodeUInt64: val :=
+    λ: "p",
+    to_u64 (!("p" +ₗ #0)) ≪ #(U64 $ 0*8) ∥
+    to_u64 (!("p" +ₗ #1)) ≪ #(U64 $ 1*8) ∥
+    to_u64 (!("p" +ₗ #2)) ≪ #(U64 $ 2*8) ∥
+    to_u64 (!("p" +ₗ #3)) ≪ #(U64 $ 3*8) ∥
+    to_u64 (!("p" +ₗ #4)) ≪ #(U64 $ 4*8) ∥
+    to_u64 (!("p" +ₗ #5)) ≪ #(U64 $ 5*8) ∥
+    to_u64 (!("p" +ₗ #6)) ≪ #(U64 $ 6*8) ∥
+    to_u64 (!("p" +ₗ #7)) ≪ #(U64 $ 7*8)
+  .
+
+  Theorem DecodeUInt64_t : (⊢ DecodeUInt64 : (arrayT byteT -> uint64T))%T.
+  Proof.
+    typecheck.
+  Qed.
+
+  Definition UInt64Put: val :=
+    λ: "p" "n",
+    EncodeUInt64 "n" (slice.ptr "p").
+
+  Theorem UInt64Put_t : ⊢ UInt64Put : (slice.T byteT -> uint64T -> unitT).
+  Proof.
+    typecheck.
+  Qed.
+
+  Definition UInt64Get: val :=
+    λ: "p",
+    DecodeUInt64 (slice.ptr "p").
+
+  Theorem UInt64Get_t : ⊢ UInt64Get : (slice.T byteT -> uint64T).
+  Proof.
+    typecheck.
+  Qed.
+
+  Definition UInt32Put: val :=
+    λ: "p" "n",
+    EncodeUInt32 "n" (slice.ptr "p").
+
+  Theorem UInt32Put_t : ⊢ UInt32Put : (slice.T byteT -> uint32T -> unitT).
+  Proof.
+    typecheck.
+  Qed.
+
+  Definition UInt32Get: val :=
+    λ: "p",
+    DecodeUInt32 (slice.ptr "p").
+
+  Theorem UInt32Get_t : ⊢ UInt32Get : (slice.T byteT -> uint32T).
+  Proof.
+    typecheck.
+  Qed.
+
+End go_lang.
+
+Hint Resolve
+     UInt64Put_t UInt64Get_t
+     UInt32Put_t UInt32Get_t : types.
